Try yet another exp_rel setup

compiler/backend/proofs/thunk_unthunkProofScript.sml
@@ -202,6 +202,11 @@ Definition is_delay_def[simp]:
   is_delay _ = F
 End
 
+Definition is_value_def[simp]:
+  is_value (Value v) = T ∧
+  is_value _ = F
+End
+
 Definition mk_case_lets_def:
   mk_case_lets f v c [] x = x ∧
   mk_case_lets f v c ((i,w)::vs) x =
@@ -217,11 +222,13 @@ Definition mk_case_rows_def:
        (mk_case_rows f v rows)
 End
 
-Overload DelayCaseLet = “mk_case_lets (Delay o Force)”;
-Overload DelayCaseRows = “mk_case_rows (Delay o Force)”;
+Overload Tick = “Letrec []”;
 
-Overload TickCaseLet = “mk_case_lets MkTick”;
-Overload TickCaseRows = “mk_case_rows MkTick”;
+Overload DelayCaseLet = “mk_case_lets (Tick o Tick o Delay o Force)”;
+Overload DelayCaseRows = “mk_case_rows (Tick o Tick o Delay o Force)”;
+
+Overload TickCaseLet = “mk_case_lets I”;
+Overload TickCaseRows = “mk_case_rows I”;
 
 Theorem mk_case_rows_neq:
   (∀f v ws n. mk_case_rows f v ws ≠ Var n) ∧
@@ -263,17 +270,31 @@ Inductive exp_rel:
      exp_rel f g ∧
      exp_rel x y ⇒
        exp_rel (App f x) (App g y)) ∧
-[exp_rel_Proj:]
-  (∀x y v i.
-     exp_rel x y ⇒
-       exp_rel (Delay (Force (Prim (Proj v i) [x])))
-               (MkTick (Prim (Proj v i) [y]))) ∧
-[exp_rel_CaseRows:]
-  (∀x y xs ys.
+[exp_rel_Case:]
+  (∀x y v xs ys.
      exp_rel x y ∧
      LIST_REL (λ(c,vs,x) (d,ws,y). c = d ∧ vs = ws ∧ exp_rel x y) xs ys ∧
-     DISJOINT (set (FLAT (MAP (FST o SND) xs))) (freevars x) ⇒
-       exp_rel (DelayCaseRows x xs) (TickCaseRows y ys)) ∧
+     DISJOINT ({v} ∪ set (FLAT (MAP (FST o SND) xs))) (freevars x) ∧
+     v ∉ set (FLAT (MAP (FST o SND) xs)) ∧
+     xs ≠ [] ⇒
+       exp_rel (Let (SOME v) (Delay x)
+                    (DelayCaseRows (Force (Var v)) xs))
+               (Let (SOME v) (Delay y)
+                    (TickCaseRows (Force (Var v)) ys))) ∧
+[exp_rel_CaseRows_Var:]
+  (∀v xs ys.
+     LIST_REL (λ(c,vs,x) (d,ws,y). c = d ∧ vs = ws ∧ exp_rel x y) xs ys ∧
+     v ∉ set (FLAT (MAP (FST o SND) xs)) ∧
+     xs ≠ [] ⇒
+       exp_rel (DelayCaseRows (Force (Var v)) xs)
+               (TickCaseRows (Force (Var v)) ys)) ∧
+[exp_rel_CaseRows_Value:]
+  (∀v w xs ys.
+     v_rel v w ∧
+     LIST_REL (λ(c,vs,x) (d,ws,y). c = d ∧ vs = ws ∧ exp_rel x y) xs ys ∧
+     xs ≠ [] ⇒
+       exp_rel (DelayCaseRows (Force (Value v)) xs)
+               (TickCaseRows (Force (Value w)) ys)) ∧
 [exp_rel_If:]
   (∀x1 y1 z1 x2 y2 z2.
      LIST_REL exp_rel [x1;y1;z1] [x2;y2;z2] ⇒
@@ -335,6 +356,12 @@ Inductive exp_rel:
   (∀x.
      v_rel (Atom x) (Atom x))
 End
+
+Theorem exp_rel_Fail[simp]:
+  exp_rel Fail Fail
+Proof
+  rw [Fail_def, Once exp_rel_cases]
+QED
 
 Theorem v_rel_def[simp]:
   (∀s x z.
@@ -451,11 +478,38 @@ Proof
   \\ simp [FILTER_FILTER, LAMBDA_PROD, AC CONJ_COMM CONJ_ASSOC]
 QED
 
-Theorem exp_rel_mk_case_lets:
+Theorem subst_Fail[simp]:
+  subst vs Fail = Fail
+Proof
+  rw [subst_def, Fail_def]
+QED
+
+Theorem mk_case_rows_subst:
+  ∀f x xs vs.
+    (∀ws x. subst ws (f x) = f (subst ws x)) ∧
+    DISJOINT (set (FLAT (MAP (FST o SND) xs))) (freevars x) ⇒
+      subst vs (mk_case_rows f x xs) =
+      mk_case_rows f (subst vs x)
+           (MAP (λ(c,ps,x). (c,ps,subst (FILTER (λ(n,x). ¬MEM n ps) vs) x)) xs)
+Proof
+  ho_match_mp_tac mk_case_rows_ind \\ rw []
+  \\ simp [mk_case_rows_def, subst_def]
+  \\ qmatch_goalsub_rename_tac ‘subst ws’
+  \\ ‘FILTER (λ(n,x). ¬MEM n vs) ws =
+      FILTER (λ(n,x). ¬MEM n (MAP SND (MAPi $, vs))) ws’
+    by simp [MAP_SND_MAPi_PROD]
+  \\ pop_assum SUBST1_TAC
+  \\ irule mk_case_lets_subst
+  \\ simp [MAP_SND_MAPi_PROD]
+QED
+
+(*
+Theorem exp_rel_mk_case_lets[local]:
   ∀f x v vs x1 g y y1.
-    exp_rel x y ∧
     exp_rel x1 y1 ∧
-    f = Delay o Force ∧
+    ((∃v. x = Force (Var v) ∧ y = Force (Var v)) ∨
+     (exp_rel x y ∧ ∃v. x = Force (Value v))) ∧
+    f = Tick o Tick o Delay o Force ∧
     g = MkTick ⇒
       exp_rel (DelayCaseLet x v vs x1) (TickCaseLet y v vs y1)
 Proof
@@ -463,19 +517,33 @@ Proof
   \\ simp [mk_case_lets_def]
   \\ irule exp_rel_Let
   \\ first_x_assum (irule_at Any) \\ gs []
-  \\ irule exp_rel_Proj \\ gs []
+  >- (
+    irule exp_rel_Proj_Var )
+  \\ qpat_x_assum ‘exp_rel (Force (Value _)) _’ mp_tac
+  \\ simp [Once exp_rel_cases, PULL_EXISTS]
+  \\ rw [Once exp_rel_cases]
+  \\ irule exp_rel_Proj_Value \\ gs []
 QED
+*)
 
-Theorem exp_rel_mk_case_lets = SIMP_RULE std_ss [] exp_rel_mk_case_lets;
-
-Theorem DelayCaseLet_subst[local] =
+Theorem DelayCaseLet_subst =
   mk_case_lets_subst
-  |> Q.SPEC ‘Delay o Force’
+  |> Q.SPEC ‘Tick o Tick o Delay o Force’
+  |> SIMP_RULE (srw_ss()) [subst_def, ELIM_UNCURRY, LET_THM];
+
+Theorem TickCaseLet_subst =
+  mk_case_lets_subst
+  |> Q.SPEC ‘I’
   |> SIMP_RULE (srw_ss()) [subst_def];
 
-Theorem TickCaseLet_subst[local] =
-  mk_case_lets_subst
-  |> Q.SPEC ‘MkTick’
+Theorem DelayCaseRows_subst =
+  mk_case_rows_subst
+  |> Q.SPEC ‘Tick o Tick o Delay o Force’
+  |> SIMP_RULE (srw_ss()) [subst_def, ELIM_UNCURRY, LET_THM];
+
+Theorem TickCaseRows_subst =
+  mk_case_rows_subst
+  |> Q.SPEC ‘I’
   |> SIMP_RULE (srw_ss()) [subst_def];
 
 Theorem exp_rel_subst:
@@ -490,44 +558,71 @@ Proof
   >- ((* Var *)
     rw [Once exp_rel_cases])
   >- ((* Prim *)
-    rw [Once exp_rel_cases]
-    >- (
-      Cases_on ‘op’ \\ gs []
-      \\ Cases_on ‘xs’ \\ gs []
-      \\ rename1 ‘DelayCaseRows x xs’
-      \\ Cases_on ‘xs’ \\ gs [mk_case_rows_def, Fail_def, subst_def,
-                              exp_rel_Prim]
-      \\ rpt (pairarg_tac \\ gvs [])
-      \\ gs [mk_case_rows_def])
-    \\ simp [subst_def]
-    \\ irule exp_rel_Prim
-    \\ simp [EVERY2_MAP]
-    \\ gvs [LIST_REL_EL_EQN] \\ rw []
-    \\ first_x_assum irule \\ fs [EL_MEM])
+    rw [Once exp_rel_cases] \\ gs []
+    >~ [‘_ (_ _ (Prim _ _)) (_ _ (Prim _ _))’] >-  (
+      simp [subst_def]
+      \\ irule exp_rel_Prim
+      \\ gs [EVERY2_MAP]
+      \\ irule LIST_REL_mono
+      \\ first_assum (irule_at Any) \\ rw [])
+    \\ first_x_assum irule \\ gs []
+    \\ (irule_at Any exp_rel_CaseRows_Var ORELSE
+        irule_at Any exp_rel_CaseRows_Value) \\ gs []
+    \\ Cases_on ‘op’ \\ Cases_on ‘xs’ \\ gs []
+    \\ rename1 ‘xs ≠ []’
+    \\ Cases_on ‘xs’ \\ gs [mk_case_rows_def]
+    \\ rpt (pairarg_tac \\ gvs [])
+    \\ gs [mk_case_rows_def])
   >- ((* If *)
-    rw [Once exp_rel_cases]
-    >- ((* Let Proj *)
-      rename1 ‘If x y z = DelayCaseRows r rs’
-      \\ rename1 ‘TickCaseRows t ts’
-      \\ Cases_on ‘rs’ \\ gs []
+    rw [Once exp_rel_cases] \\ gs []
+    >~ [‘_ (_ _ (If _ _ _)) (_ _ (If _ _ _))’] >- (
+      simp [subst_def]
+      \\ irule exp_rel_If \\ fs [])
+    \\ DEP_REWRITE_TAC [DelayCaseRows_subst]
+    \\ DEP_REWRITE_TAC [TickCaseRows_subst]
+    \\ simp [freevars_def]
+    \\ ‘MAP (FST o SND) xs = MAP (FST o SND) ys’
+      by (irule LIST_EQ
+          \\ gvs [EL_MAP, LIST_REL_EL_EQN, ELIM_UNCURRY])
+    \\ gs []
+    >- ((* CaseRows_Var *)
+      simp [subst_def]
+      \\ ‘OPTREL v_rel (ALOOKUP (REVERSE vs) v) (ALOOKUP (REVERSE ws) v)’
+        by (irule LIST_REL_OPTREL
+            \\ gs [EVERY2_MAP, LIST_REL_CONJ, ELIM_UNCURRY]
+            \\ qpat_x_assum ‘MAP FST vs = _’ mp_tac
+            \\ qid_spec_tac ‘ws’
+            \\ qid_spec_tac ‘vs’
+            \\ Induct \\ simp []
+            \\ gen_tac \\ Cases \\ simp [])
+      \\ gs [OPTREL_def]
       >- (
-        gs [mk_case_rows_def, subst_def, Fail_def])
-      \\ rpt (pairarg_tac \\ gvs [])
-      \\ gs [mk_case_rows_def]
-      \\ simp [subst_def]
-      \\ irule exp_rel_If \\ simp []
-      \\ irule_at Any exp_rel_Prim \\ simp []
-      \\ first_x_assum (irule_at Any) \\ simp []
-      \\ irule_at Any exp_rel_CaseRows \\ simp []
-      \\ last_x_assum drule
-      \\ simp [Once exp_rel_cases, PULL_EXISTS]
-      \\ disch_then drule
-      \\ simp [subst_def]
-      \\ rw [Once exp_rel_cases]
-      \\ first_x_assum (irule_at Any) \\ simp []
-      \\ irule exp_rel_mk_case_lets \\ gs [])
+        (* TODO: the substitution together with my induction hypothesis really
+         *       messes with things here *)
+        irule exp_rel_CaseRows_Var
+        \\ gs [MEM_FLAT, EVERY2_MAP, LAMBDA_PROD, MAP_MAP_o, combinTheory.o_DEF]
+        \\ irule LIST_REL_mono
+        \\ first_assum (irule_at Any)
+        \\ simp [FORALL_PROD]
+        \\ map_every qx_gen_tac [‘ctor’,‘bvs’,‘x1’,‘y1’] \\ rw []
+        \\ cheat (* TODO bleh *)
+      )
+      \\ irule exp_rel_CaseRows_Value
+      \\ gs [EVERY2_MAP, LAMBDA_PROD]
+      \\ irule LIST_REL_mono
+      \\ first_assum (irule_at Any)
+      \\ simp [FORALL_PROD]
+      \\ map_every qx_gen_tac [‘ctor’,‘bvs’,‘x1’,‘y1’] \\ rw []
+      \\ cheat (* For these cases:
+                  Use another induction theorem? *))
     \\ simp [subst_def]
-    \\ irule exp_rel_If \\ fs [])
+    \\ irule exp_rel_CaseRows_Value
+    \\ gs [EVERY2_MAP, LAMBDA_PROD]
+    \\ irule LIST_REL_mono
+    \\ first_assum (irule_at Any)
+    \\ simp [FORALL_PROD]
+    \\ map_every qx_gen_tac [‘ctor’,‘bvs’,‘x1’,‘y1’] \\ rw []
+    \\ cheat (* Same as above *))
   >- ((* App *)
     rw [Once exp_rel_cases]
     \\ simp [subst_def]
@@ -546,6 +641,19 @@ Proof
     \\ irule exp_rel_Let \\ fs [])
   >- ((* Let SOME *)
     rw [Once exp_rel_cases]
+    >- ((* Let Proj *)
+      simp [subst_def]
+      \\ qmatch_asmsub_rename_tac ‘exp_rel x1 x2’
+      \\ last_x_assum (drule_then (qspec_then ‘Delay x2’ mp_tac))
+      \\ simp [subst_def, Once exp_rel_cases, PULL_EXISTS]
+      \\ rw [Once exp_rel_cases]
+      \\ irule exp_rel_Let
+      \\ simp [Once exp_rel_cases]
+      \\ first_x_assum irule
+      \\ gs [MAP_FST_FILTER, EVERY2_MAP]
+      \\ qabbrev_tac ‘P = λx. x ≠ s’ \\ simp []
+      \\ irule_at Any LIST_REL_FILTER \\ simp []
+      \\ irule exp_rel_CaseRows_Var \\ gs [])
     \\ simp [subst_def]
     \\ irule exp_rel_Let \\ gs []
     \\ first_x_assum irule
@@ -554,42 +662,34 @@ Proof
     \\ irule LIST_REL_FILTER \\ fs [])
   >- ((* Letrec *)
     rw [Once exp_rel_cases]
-    >- (
-      Cases_on ‘xs’ \\ gs [mk_case_rows_def, Fail_def]
+    >~ [‘_ (_ _ (Letrec _ _)) (_ _ (Letrec _ _))’] >- (
+      simp [subst_def]
+      \\ ‘MAP FST f = MAP FST g’
+        by (fs [ELIM_UNCURRY, LIST_REL_CONJ]
+            \\ irule LIST_EQ
+            \\ gvs [LIST_REL_EL_EQN] \\ rw [EL_MAP])
+      \\ irule exp_rel_Letrec
+      \\ gvs [EVERY2_MAP, LAMBDA_PROD]
+      \\ first_assum (irule_at Any)
+      \\ gvs [MAP_FST_FILTER, EVERY2_MAP]
+      \\ qabbrev_tac ‘P = λx. ¬MEM x (MAP FST g)’ \\ fs []
+      \\ irule_at Any LIST_REL_FILTER \\ fs []
+      \\ irule_at Any LIST_REL_EL_MONO
+      \\ first_assum (irule_at Any) \\ rw []
       \\ rpt (pairarg_tac \\ gvs [])
-      \\ gs [mk_case_rows_def])
-    \\ simp [subst_def]
-    \\ ‘MAP FST f = MAP FST g’
-      by (fs [ELIM_UNCURRY, LIST_REL_CONJ]
-          \\ irule LIST_EQ
-          \\ gvs [LIST_REL_EL_EQN] \\ rw [EL_MAP])
-    \\ irule exp_rel_Letrec
-    \\ gvs [EVERY2_MAP, LAMBDA_PROD]
-    \\ first_assum (irule_at Any)
-    \\ gvs [MAP_FST_FILTER, EVERY2_MAP]
-    \\ qabbrev_tac ‘P = λx. ¬MEM x (MAP FST g)’ \\ fs []
-    \\ irule_at Any LIST_REL_FILTER \\ fs []
-    \\ irule_at Any LIST_REL_EL_MONO
-    \\ first_assum (irule_at Any) \\ rw []
+      \\ first_x_assum irule
+      \\ simp [MAP_FST_FILTER]
+      \\ gvs [MEM_EL, PULL_EXISTS]
+      \\ rw [Once EQ_SYM_EQ]
+      \\ first_assum (irule_at Any)
+      \\ irule_at Any LIST_REL_FILTER \\ fs [])
+    \\ Cases_on ‘xs’ \\ gs [mk_case_rows_def]
     \\ rpt (pairarg_tac \\ gvs [])
-    \\ first_x_assum irule
-    \\ simp [MAP_FST_FILTER]
-    \\ gvs [MEM_EL, PULL_EXISTS]
-    \\ rw [Once EQ_SYM_EQ]
-    \\ first_assum (irule_at Any)
-    \\ irule_at Any LIST_REL_FILTER \\ fs [])
+    \\ gs [mk_case_rows_def])
   >- ((* Delay *)
     rw [Once exp_rel_cases]
     \\ simp [subst_def, exp_rel_Value, exp_rel_Delay, SF SFY_ss]
     \\ qmatch_asmsub_abbrev_tac ‘LIST_REL R _ _’
-    >~ [‘Proj v i’] >- (
-      irule exp_rel_Proj
-      \\ first_x_assum drule
-      \\ simp [Once exp_rel_cases, PULL_EXISTS]
-      \\ simp [Once exp_rel_cases, PULL_EXISTS]
-      \\ disch_then drule
-      \\ simp [subst_def, Once exp_rel_cases]
-      \\ simp [Once exp_rel_cases])
     \\ ‘OPTREL R (ALOOKUP (REVERSE vs) v) (ALOOKUP (REVERSE ws) v)’
       by (irule LIST_REL_OPTREL
           \\ gvs [EVERY2_MAP, ELIM_UNCURRY, LIST_REL_CONJ, Abbr ‘R’]
@@ -709,18 +809,12 @@ Proof
     \\ first_x_assum (drule_all_then strip_assume_tac)
     \\ Cases_on ‘eval_to k x1’ \\ Cases_on ‘eval_to k g’ \\ gs []
     \\ qpat_x_assum ‘exp_rel (Delay _) _’ mp_tac
-    \\ rw [Once exp_rel_cases] \\ gs [eval_to_def]
+    \\ rw [Once exp_rel_cases]
+    >~ [‘Force (Var v)’] >- (
+      gs [closed_def])
+    \\ gs [eval_to_def]
     \\ rename1 ‘dest_anyClosure v1’
     \\ rename1 ‘v_rel v1 v2’
-    >~ [‘Prim (Proj v i) [x]’] >- (
-      Cases_on ‘k = 0’ \\ gs []
-      \\ rename1 ‘exp_rel x y’
-      \\ Cases_on ‘eval_to (k - 1) y’ \\ gs []
-      \\ rename1 ‘eval_to (k - 1) y = INR w’
-      \\ Cases_on ‘dest_Constructor w’ \\ gs []
-      \\ rpt (pairarg_tac \\ gvs [])
-      \\ qpat_x_assum ‘(_ +++ _) _ _’ mp_tac
-      \\ IF_CASES_TAC \\ gs [])
     THEN (
       Cases_on ‘v1’ \\ Cases_on ‘v2’ \\ gvs [dest_anyClosure_def]
       >- ((* Thunk-Thunk *)
@@ -761,6 +855,40 @@ Proof
     \\ Cases_on ‘eval_to (k - 1) x1’ \\ Cases_on ‘eval_to (k - 1) x2’ \\ gs [])
   >- ((* Let SOME *)
     rw [Once exp_rel_cases]
+    >- ((* Let Proj *)
+      simp [eval_to_def]
+      \\ gs [exp_inv_def]
+      \\ IF_CASES_TAC \\ gs []
+      \\ first_x_assum irule
+      \\ simp [closed_subst, exp_inv_subst]
+      \\ DEP_REWRITE_TAC [DelayCaseRows_subst]
+      \\ DEP_REWRITE_TAC [TickCaseRows_subst]
+      \\ gs [freevars_def]
+      \\ ‘MAP (FST o SND) ys = MAP (FST o SND) xs’
+        by (irule LIST_EQ
+            \\ gvs [LIST_REL_EL_EQN, EL_MAP, ELIM_UNCURRY])
+      \\ simp []
+      \\ qmatch_goalsub_abbrev_tac ‘MAP f xs’
+      \\ qmatch_goalsub_abbrev_tac ‘MAP g ys’
+      \\ qmatch_asmsub_rename_tac ‘exp_rel x1 x2’
+      \\ ‘MAP f xs = MAP (λ(a,b,c). (a,b,subst [(n, Thunk (INR x1))] c)) xs’
+        by (gs [MAP_EQ_f, Abbr ‘f’, MEM_FLAT, ELIM_UNCURRY] \\ rw []
+            \\ gs [MEM_MAP, DISJ_EQ_IMP, PULL_EXISTS])
+      \\ pop_assum SUBST1_TAC
+      \\ ‘MAP g ys = MAP (λ(a,b,c). (a,b,subst [(n, Thunk (INR x2))] c)) ys’
+        by (‘¬MEM n (FLAT (MAP (FST o SND) ys))’ by gs []
+            \\ qpat_x_assum ‘MAP _ ys = _’ kall_tac
+            \\ qpat_x_assum ‘¬MEM n (FLAT (MAP _ xs))’ kall_tac
+            \\ gs [MAP_EQ_f, Abbr ‘g’, MEM_FLAT, ELIM_UNCURRY] \\ rw []
+            \\ gs [MEM_MAP, DISJ_EQ_IMP, PULL_EXISTS])
+      \\ pop_assum SUBST1_TAC
+      \\ simp [subst1_def]
+      \\ irule exp_rel_CaseRows_Value
+      \\ gs [EVERY2_MAP, LAMBDA_PROD]
+      \\ irule LIST_REL_mono
+      \\ first_assum (irule_at Any)
+      \\ simp [FORALL_PROD] \\ rw []
+      \\ irule exp_rel_subst \\ gs [])
     \\ gvs [exp_inv_def]
     \\ rename1 ‘exp_rel x1 x2’
     \\ rename1 ‘exp_rel y1 y2’
@@ -772,84 +900,45 @@ Proof
     \\ irule_at Any exp_rel_subst \\ gs [])
   >- ((* If *)
     rw [Once exp_rel_cases] \\ fs [exp_inv_def]
-    >- ((* Let Proj *)
-      Cases_on ‘xs’ \\ gs [mk_case_rows_def, Fail_def]
-      \\ rpt (pairarg_tac \\ gvs [])
-      \\ gvs [mk_case_rows_def, exp_inv_def]
-      \\ simp [eval_to_def]
+    >~ [‘_ (_ _ (If _ _ _)) (_ _ (If _ _ _))’] >- (
+      rename1 ‘If x y z’
+      \\ rw [eval_to_def] \\ gvs [exp_inv_def]
+      \\ first_x_assum (drule_then assume_tac) \\ fs []
+      \\ first_x_assum (drule_then assume_tac) \\ fs []
+      \\ first_x_assum (drule_then assume_tac) \\ fs []
+      \\ Cases_on ‘eval_to (k - 1) x’ \\ Cases_on ‘eval_to (k - 1) x2’ \\ gs []
       \\ IF_CASES_TAC \\ gs []
       \\ IF_CASES_TAC \\ gs []
-      \\ qpat_x_assum ‘∀x. exp_rel (Prim _ _) _ ⇒ _’ mp_tac
-      \\ simp [Once exp_rel_cases, PULL_EXISTS]
-      \\ disch_then (drule_then assume_tac)
-      \\ gs [eval_to_def]
-      \\ Cases_on ‘eval_to (k - 2) x'''’ \\ gs []
-      >- (
-        Cases_on ‘eval_to (k - 2) y'’ \\ gs []
-        \\ Cases_on ‘dest_Constructor y’ \\ gs []
-        \\ pairarg_tac \\ gvs []
-        \\ IF_CASES_TAC \\ gs [])
-      \\ Cases_on ‘dest_Constructor y’ \\ gs []
-      >- (
-        Cases_on ‘eval_to (k - 2) y'’ \\ gs []
-        \\ Cases_on ‘dest_Constructor y'''’ \\ gs []
-        \\ pairarg_tac \\ gvs []
-        \\ IF_CASES_TAC \\ gs [])
-      \\ pairarg_tac \\ gvs []
       \\ IF_CASES_TAC \\ gs []
-      >- (
-        Cases_on ‘eval_to (k - 2) y'’ \\ gs []
-        \\ Cases_on ‘dest_Constructor y'''’ \\ gs []
-        \\ pairarg_tac \\ gvs []
-        \\ gs [CaseEq "bool"]
-        \\ IF_CASES_TAC \\ gs []
-        >- (
-          IF_CASES_TAC \\ gs []
-          \\ gvs [CaseEq "bool"]
-          \\ first_x_assum (irule_at Any)
-          \\ irule exp_rel_mk_case_lets \\ gs [])
-        \\ IF_CASES_TAC \\ gs []
-        \\ gs [CaseEq "bool"]
-        \\ first_x_assum (irule_at Any)
-        \\ irule exp_rel_CaseRows \\ gs [])
-      \\ Cases_on ‘eval_to (k - 2) y'’ \\ gs []
-      \\ Cases_on ‘dest_Constructor y'''’ \\ gs []
-      \\ pairarg_tac \\ gvs []
       \\ IF_CASES_TAC \\ gs [])
-    \\ rename1 ‘If x y z’
-    \\ rw [eval_to_def] \\ gvs [exp_inv_def]
-    \\ first_x_assum (drule_then assume_tac) \\ fs []
-    \\ first_x_assum (drule_then assume_tac) \\ fs []
-    \\ first_x_assum (drule_then assume_tac) \\ fs []
-    \\ Cases_on ‘eval_to (k - 1) x’ \\ Cases_on ‘eval_to (k - 1) x2’ \\ gs []
-    \\ IF_CASES_TAC \\ gs []
-    \\ IF_CASES_TAC \\ gs []
-    \\ IF_CASES_TAC \\ gs []
-    \\ IF_CASES_TAC \\ gs [])
+    >- ((* Var *)
+      Cases_on ‘xs’ \\ gs [mk_case_rows_def]
+      \\ rpt (pairarg_tac \\ gvs [])
+      \\ gvs [mk_case_rows_def])
+    \\ cheat
+       (* ... (eval_to k (DelayCaseRows ...)) (eval_to k(TickCaseRows ...)) *))
   >- ((* Letrec *)
     rw [Once exp_rel_cases]
-    >- ((* Fail *)
-      Cases_on ‘xs’ \\ gs [mk_case_rows_def, Fail_def]
-      \\ rpt (pairarg_tac \\ gvs [])
-      \\ gs [mk_case_rows_def])
-    \\ rw [eval_to_def] \\ gvs [exp_inv_def]
-    \\ first_x_assum irule
-    \\ simp [subst_funs_def, closed_subst]
-    \\ irule_at Any exp_rel_subst
-    \\ irule_at Any exp_inv_subst
-    \\ irule_at Any LIST_EQ
-    \\ gs [MAP_MAP_o, combinTheory.o_DEF, LAMBDA_PROD, SUBSET_DIFF_EMPTY,
-           GSYM FST_THM, EL_MAP, EVERY_MAP, SF CONJ_ss]
-    \\ gs [ELIM_UNCURRY]
-    \\ gvs [LIST_REL_EL_EQN, EL_MAP, BIGUNION_SUBSET, MEM_MAP, PULL_EXISTS,
-            freevars_def, MEM_EL]
-    \\ rw [ELIM_UNCURRY, freevars_def, MAP_MAP_o, combinTheory.o_DEF,
-           SF ETA_ss])
+    >~ [‘_ (_ _ (Letrec _ _)) (_ _ (Letrec _ _))’] >- (
+      rw [eval_to_def] \\ gvs [exp_inv_def]
+      \\ first_x_assum irule
+      \\ simp [subst_funs_def, closed_subst]
+      \\ irule_at Any exp_rel_subst
+      \\ irule_at Any exp_inv_subst
+      \\ irule_at Any LIST_EQ
+      \\ gs [MAP_MAP_o, combinTheory.o_DEF, LAMBDA_PROD, SUBSET_DIFF_EMPTY,
+             GSYM FST_THM, EL_MAP, EVERY_MAP, SF CONJ_ss]
+      \\ gs [ELIM_UNCURRY]
+      \\ gvs [LIST_REL_EL_EQN, EL_MAP, BIGUNION_SUBSET, MEM_MAP, PULL_EXISTS,
+              freevars_def, MEM_EL]
+      \\ rw [ELIM_UNCURRY, freevars_def, MAP_MAP_o, combinTheory.o_DEF,
+             SF ETA_ss])
+    \\ Cases_on ‘xs’ \\ gs [mk_case_rows_def]
+    \\ rpt (pairarg_tac \\ gvs [])
+    \\ gvs [mk_case_rows_def])
   >- ((* Delay *)
-    rw [Once exp_rel_cases] \\ gs [eval_to_def, exp_inv_def, v_rel_Thunk_Same]
-    \\ cheat (* The left side needs to tick, and we can't have something fail
-                on the right side, so it would be good if we can make it a
-                value *))
+    rw [Once exp_rel_cases]
+    \\ gs [eval_to_def, exp_inv_def, v_rel_Thunk_Same])
   >- ((* Box *)
     rw [Once exp_rel_cases])
   >- ((* Force *)
@@ -958,13 +1047,14 @@ Proof
     rw [Once exp_rel_cases])
   >- ((* Prim *)
     rw [Once exp_rel_cases]
-    >- ((* Fail *)
+    \\ TRY ((* Fail *)
       Cases_on ‘op’ \\ gs []
       \\ Cases_on ‘xs’ \\ gs []
       \\ rename1 ‘DelayCaseRows x xs’
       \\ Cases_on ‘xs’ \\ gs [mk_case_rows_def, Fail_def, eval_to_def]
       \\ rpt (pairarg_tac \\ gvs [])
-      \\ gs [mk_case_rows_def])
+      \\ gs [mk_case_rows_def]
+      \\ NO_TAC)
     \\ gvs []
     \\ simp [eval_to_def]
     \\ Cases_on ‘op’ \\ gs [exp_inv_def, EVERY_EL, EL_MAP, LIST_REL_EL_EQN]
